Add AES canright and canright_masked_noreuse sboxes (#149)
- Currently compiles but is untested

cava/arrow-examples/Aes/canright_pkg.v
@@ -5,7 +5,7 @@ From Coq Require Import NArith Lia.
 
 Import KappaNotation.
 
-From Aes Require Import Util.
+Require Import Util pkg.
 
 Section var.
 Variable var: Kind -> Kind -> Type.
@@ -26,8 +26,8 @@ Definition aes_mul_gf2p2
   : kappa_sugared var << Vector 2 Bit , Vector 2 Bit , Unit >> << Vector 2 Bit>> :=
 <[ \g d =>
   let a = and (g[#1]) (d[#1]) in
-  let g_xor = !(reduce Xor) g in
-  let d_xor = !(reduce Xor) d in
+  let g_xor = !(reduce _ Xor) g in
+  let d_xor = !(reduce _ Xor) d in
   let b = and g_xor d_xor in
   let c = and (g[#0]) (d[#0]) in
   mkVec
@@ -104,13 +104,12 @@ Definition aes_mul_gf2p4
 refine (
 <[ \gamma delta =>
   let a = !aes_mul_gf2p2 (gamma[3:2]) (delta[3:2]) in
-  let b = !aes_mul_gf2p2 (!map2_xor (gamma[3:2]) (gamma[1:0])) (!map2_xor (delta[3:2]) (delta[1:0])) in
+  let b = !aes_mul_gf2p2 (gamma[3:2] ^ gamma[1:0]) (delta[3:2] ^ delta[1:0]) in
   let c = !aes_mul_gf2p2 (gamma[1:0]) (delta[1:0]) in
   concat
-    (!map2_xor c (!aes_scale_omega2_gf2p2 b))
-    (!map2_xor a (!aes_scale_omega2_gf2p2 b))
-]>);
-  abstract lia.
+    (c ^ !aes_scale_omega2_gf2p2 b)
+    (a ^ !aes_scale_omega2_gf2p2 b)
+]>); compute; auto.
 Defined.
 
 (* // Square and scale by nu in GF(2^4)/GF(2^2), using normal basis [alpha^8, alpha^2] *)
@@ -128,13 +127,12 @@ Definition aes_square_scale_gf2p4_gf2p2
   : kappa_sugared var << Vector 4 Bit, Unit >> << Vector 4 Bit >>.
 refine (
 <[ \gamma =>
-    let a = !map2_xor (gamma[3:2]) (gamma[1:0]) in
+    let a = gamma[3:2] ^ gamma[1:0] in
     let b = !aes_square_gf2p2 (gamma[1:0]) in
     concat
       (!aes_scale_omega_gf2p2 b)
       (!aes_square_gf2p2 a)
-]>);
-  abstract lia.
+]>); compute; auto.
 Defined.
 
 (* // Basis conversion matrices to convert between polynomial basis A, normal basis X *)
@@ -145,16 +143,104 @@ Defined.
 (* // transformation from polynomial basis A to normal basis X. *)
 (* // (see Appendix A of the technical report) *)
 (* parameter logic [7:0] A2X [8] = '{8'h98, 8'hf3, 8'hf2, 8'h48, 8'h09, 8'h81, 8'ha9, 8'hff}; *)
+Definition A2X : kappa_sugared var Unit (Vector 8 (Vector 8 Bit)) :=
+  <[ mkVec 
+    ( #255 (* = Byte.xff, coq doesn't have hex literals? *)
+    , #169 (* 0xa9 *)
+    , #129 (* 0x81 *)
+    , #  9 (* 0x09 *)
+    , # 72 (* 0x48 *)
+    , #242 (* 0xf2 *)
+    , #243 (* 0xf3 *)
+    , #152 (* 0x98 *)
+    )
+  ]>.
 (* parameter logic [7:0] X2A [8] = '{8'h64, 8'h78, 8'h6e, 8'h8c, 8'h68, 8'h29, 8'hde, 8'h60}; *)
+Definition X2A : kappa_sugared var Unit (Vector 8 (Vector 8 Bit)) :=
+  <[ mkVec 
+    ( #  6 (* 0x06 *)
+    , #222 (* 0xde *)
+    , # 41 (* 0x29 *)
+    , #104 (* 0x68 *)
+    , #140 (* 0x8c *)
+    , #110 (* 0x6e *)
+    , #120 (* 0x78 *)
+    , #100 (* 0x64 *)
+    )
+  ]>.
 (* parameter logic [7:0] X2S [8] = '{8'h58, 8'h2d, 8'h9e, 8'h0b, 8'hdc, 8'h04, 8'h03, 8'h24}; *)
+Definition X2S : kappa_sugared var Unit (Vector 8 (Vector 8 Bit)) :=
+  <[ mkVec 
+    ( # 36 (* 0x24 *)
+    , #  3 (* 0x03 *)
+    , #  4 (* 0x04 *)
+    , #220 (* 0xdc *)
+    , # 11 (* 0x0b *)
+    , #158 (* 0x9e *)
+    , # 45 (* 0x2d *)
+    , # 88 (* 0x58 *)
+    )
+  ]>.
 (* parameter logic [7:0] S2X [8] = '{8'h8c, 8'h79, 8'h05, 8'heb, 8'h12, 8'h04, 8'h51, 8'h53}; *)
+Definition S2X : kappa_sugared var Unit (Vector 8 (Vector 8 Bit)) :=
+  <[ mkVec 
+    ( # 83 (* 0x53 *)
+    , # 81 (* 0x51 *)
+    , #  4 (* 0x04 *)
+    , # 18 (* 0x12 *)
+    , #235 (* 0xeb *)
+    , #  5 (* 0x05 *)
+    , #121 (* 0x79 *)
+    , #140 (* 0x8c *)
+    )
+  ]>.
 
 End var.
 
 Section sanity_check.
-  Lemma aes_mul_gf2p4_wf: wf_debrujin ENil (Desugar aes_mul_gf2p4 natvar).
-  Proof. exact (Kappa_wf (Desugar (@aes_mul_gf2p4))). Qed.
+  Lemma aes_mul_gf2p2_wf: wf_debrujin ENil (Desugar (aes_mul_gf2p2) _).
+  Proof. wf_kappa_via_compute. Defined.
 
-  Definition aes_mul_gf2p4_structure: structure << Vector 4 Bit, Vector 4 Bit >> << Vector 4 Bit >>
+  Lemma aes_mul_gf2p4_wf: wf_debrujin ENil (Desugar (aes_mul_gf2p4) _).
+  Proof. wf_kappa_via_compute. Qed.
+
+  Lemma aes_square_scale_gf2p4_gf2p2_wf: wf_debrujin ENil (Desugar (aes_square_scale_gf2p4_gf2p2) _).
+  Proof. wf_kappa_via_compute. Qed.
+
+  Definition aes_mul_gf2p2_structure
+    := to_constructive (Desugar (@aes_mul_gf2p2)) aes_mul_gf2p2_wf.
+
+  Definition aes_mul_gf2p4_structure
     := to_constructive (Desugar (@aes_mul_gf2p4)) aes_mul_gf2p4_wf.
+
+  Definition aes_square_scale_gf2p4_gf2p2_structure
+    := to_constructive (Desugar (@aes_square_scale_gf2p4_gf2p2)) aes_square_scale_gf2p4_gf2p2_wf.
+
+  (* Eval compute in aes_square_scale_gf2p4_gf2p2_structure.
+  Eval compute in aes_mul_gf2p2_structure. *)
+
+
+  Ltac debug_match tac x :=
+    match x with
+    | context[match ?X with |eq_refl => ?Y end] => tac
+    end.
+
+Require Import Cava.Arrow.Instances.Prop.
+
+  Goal toCava aes_mul_gf2p2_structure NoLoops.
+    compute.
+    tauto.
+  Qed.
+
 End sanity_check.
+
+Arguments aes_scale_omega_gf2p2 {var}. 
+Arguments aes_scale_omega2_gf2p2 {var}. 
+Arguments aes_square_gf2p2 {var}. 
+Arguments aes_mul_gf2p2 {var}. 
+Arguments aes_mul_gf2p4 {var}. 
+Arguments aes_square_scale_gf2p4_gf2p2 {var}. 
+Arguments A2X {var}. 
+Arguments S2X {var}. 
+Arguments X2S {var}. 
+Arguments X2A {var}. 
