cava/arrow-examples/Aes/Pkg.v
@@ -1,155 +1,50 @@
-(* TODO:
-
-An aspirational direct translation to work towards. Currently not working.
-
-*)
-Require Import Cava.Netlist.
-
+Require Import Cava.Arrow.Kappa.Syntax.
 Require Import Cava.Arrow.Arrow.
-Require Import Cava.Arrow.Syntax.
 
-Open Scope source.
+From Coq Require Import NArith Lia.
 
-(* function automatic logic [7:0] aes_mul2(logic [7:0] in); *)
-(*   logic [7:0] out; *)
-(*   out[7] = in[6]; *)
-(*   out[6] = in[5]; *)
-(*   out[5] = in[4]; *)
-(*   out[4] = in[3] ^ in[7]; *)
-(*   out[3] = in[2] ^ in[7]; *)
-(*   out[2] = in[1]; *)
-(*   out[1] = in[0] ^ in[7]; *)
-(*   out[0] = in[7]; *)
-(*   return out; *)
-(* endfunction *)
-Definition aes_mult2
-  : Kappa (bitvec [8] ** unit) (bitvec [8]) := <[
-  \x =>
-  bitvec
-    ( x[6]
-    , x[5]
-    , x[4]
-    , x[3] ^ x[7]
-    , x[2] ^ x[7]
-    , x[1]
-    , x[0] ^ x[7]
-    , x[7]
-    )
-]>.
+Import KappaNotation.
 
-Definition aes_mult4
-  : Kappa (bitvec [8] ** unit) (bitvec [8]) := <[
-  \x => aes_mul2 (aes_mul2 x)
-]>.
+Require Import Util List.
 
-(* function automatic logic [7:0] aes_div2(logic [7:0] in); *)
-(*   logic [7:0] out; *)
-(*   out[7] = in[0]; *)
-(*   out[6] = in[7]; *)
-(*   out[5] = in[6]; *)
-(*   out[4] = in[5]; *)
-(*   out[3] = in[4] ^ in[0]; *)
-(*   out[2] = in[3] ^ in[0]; *)
-(*   out[1] = in[2]; *)
-(*   out[0] = in[1] ^ in[0]; *)
-(*   return out; *)
-(* endfunction *)
-Definition aes_div2
-  : Kappa (bitvec [8] ** unit) (bitvec [8]) := <[
-  \x =>
-  bitvec
-    ( x[0]
-    , x[7]
-    , x[6]
-    , x[5]
-    , x[4] ^ x[0]
-    , x[3] ^ x[0]
-    , x[2]
-    , x[1] ^ x[0]
-    )
-]>.
+Section var.
+Variable var: Kind -> Kind -> Type.
 
-(* function automatic logic [31:0] aes_circ_byte_shift(logic [31:0] in, logic [1:0] shift); *)
-(*   logic [31:0] out; *)
-(*   logic [31:0] s; *)
-(*   s = {30'b0,shift}; *)
-(*   out = {in[8*((7-s)%4) +: 8], in[8*((6-s)%4) +: 8], *)
-(*          in[8*((5-s)%4) +: 8], in[8*((4-s)%4) +: 8]}; *)
-(*   return out; *)
-(* endfunction *)
-Definition aes_circ_byte_shift
-  : Kappa (bitvec [32] ** bitvec [2] ** unit) (bitvec [32]) := <[
-  \value shift =>
-  let s = concat ( 0 : bitvec 30 ) shift in
-  concat
-    (concat
-      value[8*((7-s)%4) +: 8]
-      value[8*((6-s)%4) +: 8])
-    (concat
-      value[8*((5-s)%4) +: 8]
-      value[8*((4-s)%4) +: 8])
-]>.
+(* typedef enum logic {
+  CIPH_FWD = 1'b0,
+  CIPH_INV = 1'b1
+} ciph_op_e; *)
+Definition CIPH_FWD {n} : kappa_sugared var Unit (Vector n Bit) := <[ #0 ]>.
+Definition CIPH_INV {n} : kappa_sugared var Unit (Vector n Bit) := <[ #1 ]>.
 
-(* function automatic logic [3:0][3:0][7:0] aes_transpose(logic [3:0][3:0][7:0] in); *)
-(*   logic [3:0][3:0][7:0] transpose; *)
-(*   transpose = '0; *)
-(*   for (int j=0; j<4; j++) begin *)
-(*     for (int i=0; i<4; i++) begin *)
-(*       transpose[i][j] = in[j][i]; *)
-(*     end *)
-(*   end *)
-(*   return transpose; *)
-(* endfunction *)
-Definition aes_transpose 
-  : Kappa (bitvec [4;4;8] ** unit) (bitvec [4;4;8]) := 
-  reshape (concat_bitvec
-  (map (fun j => 
-    map (fun i => 
-      <[ \x => x[j][i] ]>.
-    ) (seq 0 4)
-  ) (seq 0 4)
-  )
-  ).
-
-
-(* function automatic logic [3:0][7:0] aes_col_get(logic [3:0][3:0][7:0] in, logic [1:0] idx); *)
-(*   logic [3:0][7:0] out; *)
-(*   for (int i=0; i<4; i++) begin *)
-(*     out[i] = in[i][idx]; *)
-(*   end *)
-(*   return out; *)
-(* endfunction *)
-Definition aes_col_get 
-  : Kappa (bitvec [4;4;8] ** bitvec[2] ** unit) (bitvec [4;8]) := 
-
-  concat_bitvec
-  (map (fun j => 
-      <[ \x idx => x[j][idx] ]>.
-  ) (seq 0 4)
-  ).
-
-(* function automatic logic [7:0] aes_mvm( *)
-(*   logic [7:0] vec_b, *)
-(*   logic [7:0] mat_a [8] *)
-(* ); *)
-(*   logic [7:0] vec_c; *)
-(*   vec_c = '0; *)
-(*   for (int i=0; i<8; i++) begin *)
-(*     for (int j=0; j<8; j++) begin *)
-(*       vec_c[i] = vec_c[i] ^ (mat_a[j][i] & vec_b[7-j]); *)
-(*     end *)
-(*   end *)
-(*   return vec_c; *)
-(* endfunction *)
+Fixpoint outer {n}
+  : kappa_sugared var <<Bit, Unit>> (Vector (S n) Bit) := 
+match n with
+| 0 => <[ \x => mkVec (x) ]>
+| S n => <[ \x => x :: !outer x ]>
+end.
 
 Definition aes_mvm_acc
-  (j: bitvec [3])
-  : Kappa (bitvec [8] ** bitvec[8][8] ** bitvec[8] ** unit) (bitvec [8]) := 
-  (map (fun i => 
-      <[ \vector matrix acc => acc[i] ^ (matrix[j][i] & vector[7-j]) ]>.
-  ) (seq 0 4)
-  ).
+  : kappa_sugared var <<Vector 8 Bit, Vector 8 Bit, Bit, Unit>> (Vector 8 Bit) := 
+  <[\acc mat vec => acc ^ (mat & (!outer vec)) ]>.
 
-Definition aes_mvm
-  : Kappa (bitvec [8] ** bitvect [8][8] ** unit) (bitvec [8]) := 
-  fold (fun i acc => aes_mvm_acc i) <[constant_vec 0]> (seq 0 4).
+Definition aes_mvm: kappa_sugared var <<Vector 8 Bit, Vector 8 (Vector 8 Bit), Unit>> (Vector 8 Bit) :=
+  <[\ vec_b mat_a =>
+  let _1 = !aes_mvm_acc (#0) (mat_a[#0]) (vec_b[#7]) in
+  let _2 = !aes_mvm_acc (_1) (mat_a[#1]) (vec_b[#6]) in
+  let _3 = !aes_mvm_acc (_2) (mat_a[#2]) (vec_b[#5]) in
+  let _4 = !aes_mvm_acc (_3) (mat_a[#3]) (vec_b[#4]) in
+  let _5 = !aes_mvm_acc (_4) (mat_a[#4]) (vec_b[#3]) in
+  let _6 = !aes_mvm_acc (_5) (mat_a[#5]) (vec_b[#2]) in
+  let _7 = !aes_mvm_acc (_6) (mat_a[#6]) (vec_b[#1]) in
+  let _8 = !aes_mvm_acc (_7) (mat_a[#7]) (vec_b[#0]) in
+  _8
+  ]>.
+
+End var.
+
+
+Arguments aes_mvm {var}. 
+Arguments outer {var}. 
+Arguments CIPH_FWD {var n}. 
+Arguments CIPH_INV {var n}. 
