cava/cava/Cava/Arrow/Kappa/Kappa.v
@@ -1,12 +1,13 @@
 Require Import Cava.Arrow.Arrow.
 Require Import Cava.Arrow.Instances.Constructive.
 
-From Coq Require Import Arith NArith Lia.
+From Coq Require Import Arith NArith Lia NaryFunctions.
 
 Section Vars.
   Context {var: Kind -> Kind -> Type}.
 
-  (* `kappa_sugared` includes constructors for 
+  (* 
+    `kappa_sugared` includes constructors for 
     - Kappa Calculus, 
     - the Cava methods, 
     - lifting any morphism from the Constructive arrow instance, 
@@ -16,6 +17,7 @@ Section Vars.
     "primitive"/required constructors, the rest are a to help syntax 
     or type inference and desugar simply to combinations of the others.
     *)
+  (* TODO: cleanup / have a more modular EDSL representation *)
   Inductive kappa_sugared : Kind -> Kind -> Type :=
     (* Kappa Calculus *)
     | Var: forall {x y},    var x y -> kappa_sugared x y
@@ -47,9 +49,8 @@ Section Vars.
     | Xorcy: kappa_sugared << Bit, Bit, Unit >> Bit
     | Muxcy: kappa_sugared << Bit, Tuple Bit Bit, Unit >> Bit
     | UnsignedAdd: forall a b c, kappa_sugared << Vector a Bit, Vector b Bit, Unit >> (Vector c Bit)
-    (* TODO: enable lut *)
-    (*| Lut n: (bool^^n --> bool) -> bitvec (N.of_nat n) ~> bit;*)
-    | IndexVec: forall n {o}, kappa_sugared << Vector n o, Vector (Nat.log2_up n) Bit, Unit >> o
+    | Lut n: (bool^^n --> bool) -> kappa_sugared << Vector n Bit, Unit >> Bit
+    | IndexVec: forall n {o}, kappa_sugared << Vector n o, Vector (log2_up_min_1 n) Bit, Unit >> o
     | SliceVec: forall n x y {o}, x < n -> y <= x -> kappa_sugared << Vector n o, Unit >> (Vector (x - y + 1) o)
     | ToVec: forall {o}, kappa_sugared << o, Unit >> (Vector 1 o)
     | Append: forall n {o}, kappa_sugared << Vector n o, o, Unit >> (Vector (n+1) o)
@@ -97,7 +98,7 @@ Section Vars.
 
   Definition kappa_index_vec {n o}
     (array: kappa_sugared Unit (Vector n o))
-    (index: kappa_sugared Unit (Vector (Nat.log2_up n) Bit))
+    (index: kappa_sugared Unit (Vector (log2_up_min_1 n) Bit))
     : kappa_sugared Unit o :=
     (App (App (IndexVec n) array) index).
 
@@ -124,11 +125,15 @@ Section Vars.
     let tail_ := Let (App TupleRight circuit) (fun x => Var x) in
     _).
     assert ((S (S n)) - 1 = S n).
-    lia.
+    simpl. auto.
     rewrite H in tail_.
     exact ( tupleHelper head_ tail_ ).
     Grab Existential Variables.
-    abstract lia.
+    compute.
+    auto.
+    apply le_n_S.
+    apply le_n_S.
+    apply le_0_n.
   Defined.
   Definition kappa_head' {n o}
     : kappa_sugared << Vector (S (S n)) o, Unit>> <<o, Vector (S n) o>>
@@ -162,12 +167,13 @@ Section Vars.
     | Xorcy  => kappa_app << Bit, Bit, Unit >> xorcy 
     | Muxcy  => kappa_app << Bit, Tuple Bit Bit, Unit >> muxcy 
     | UnsignedAdd a b c => kappa_app << Vector a Bit, Vector b Bit, Unit >> (unsigned_add a b c)
+    | Lut n f => kappa_app << Vector n Bit, Unit >> (lut n f)
 
     | Constant b => DArr (constant b)
     | ConstantVec v => DArr (constant_bitvec _ v)
 
     | IndexVec n => 
-      kappa_app << Vector n _, Vector (Nat.log2_up n) Bit, Unit >> (index_vec n _)
+      kappa_app << Vector n _, Vector (log2_up_min_1 n) Bit, Unit >> (index_vec n _)
     | SliceVec n x y H1 H2 => 
       kappa_app << Vector n _, Unit >> (slice_vec n x y _ H1 H2)
 
